prototype format for ownership invariants

messageInvariantPrototypes/shardedKvBatched/distributedMonotonic/applicationProof.dfy
@@ -1,4 +1,5 @@
 include "messageInvariants.dfy"
+include "uniquenessInvariants.dfy"
 
 module ShardedKVProof {
   import opened Types
@@ -6,6 +7,7 @@ module ShardedKVProof {
   import opened DistributedSystem
   import opened Obligations
   import opened MessageInvariants
+  import opened UniquenessInvariants
 
   ghost predicate HostsCompleteKeys(c: Constants, v: Variables)
    requires v.WF(c)
@@ -15,57 +17,18 @@ module ShardedKVProof {
       && c.ValidIdx(idx)
     :: v.History(i).hosts[idx].HasKey(k)
   }
-
-  ghost predicate KeyInFlight(c: Constants, v: Variables, k: UniqueKey) 
-    requires v.WF(c)
-  {
-    exists msg :: KeyInFlightByMessage(c, v, msg, k)
-  }
-
-  ghost predicate KeyInFlightByMessage(c: Constants, v: Variables, msg: Message, k: UniqueKey) 
-    requires v.WF(c)
-  {
-    && msg in v.network.sentMsgs
-    && (0 <= msg.Dst() < |c.hosts| ==>
-      Host.UniqueKeyInFlight(c.hosts[msg.Dst()], v.Last().hosts[msg.Dst()], k, msg)
-    )
-  }
-
-  ghost predicate AtMostOneInFlight(c: Constants, v: Variables)
-    requires v.WF(c)
-  {
-    forall k, m1, m2 | KeyInFlightByMessage(c, v, m1, k) && KeyInFlightByMessage(c, v, m2, k) 
-    :: m1 == m2
-  }
-
-  ghost predicate NoneHasLiveKey(c: Constants, v: Variables, k: UniqueKey) 
-    requires v.WF(c)
-  {
-    forall idx | c.ValidIdx(idx) :: !v.Last().hosts[idx].HasLiveKey(k)
-  }
-  
-
-  ghost predicate LiveKeyImpliesNoneInFlight(c: Constants, v: Variables)
-    requires v.WF(c)
-  {
-    forall k | !NoneHasLiveKey(c, v, k)
-    ::
-    !KeyInFlight(c, v, k)
-  }
-
   
   ghost predicate ApplicationInv(c: Constants, v: Variables)
     requires v.WF(c)
   {
     && HostsCompleteKeys (c, v)
-    && AtMostOneInFlight(c, v)
-    && LiveKeyImpliesNoneInFlight(c, v)
   }
 
   ghost predicate Inv(c: Constants, v: Variables)
   {
     && v.WF(c)
     && MessageInv(c, v)
+    && UniquenessInv(c, v)
     && ApplicationInv(c, v)
     && Safety(c, v)
   }
@@ -80,6 +43,7 @@ module ShardedKVProof {
     ensures Inv(c, v)
   {
     InitImpliesMessageInv(c, v);
+    InitImpliesUniquenessInv(c, v);
   }
 
   lemma InvInductive(c: Constants, v: Variables, v': Variables)
@@ -88,9 +52,8 @@ module ShardedKVProof {
     ensures Inv(c, v')
   {
     MessageInvInductive(c, v, v');
+    UniquenessInvInductive(c, v, v');
     InvNextHostsCompleteKeys(c, v, v');
-    InvNextAtMostOneInFlight(c, v, v');
-    InvNextLiveKeyImpliesNoneInFlight(c, v, v');
     InvNextSafety(c, v, v');
   }
 
@@ -117,71 +80,6 @@ lemma InvNextHostsCompleteKeys(c: Constants, v: Variables, v': Variables)
       var actor, msgOps := dsStep.actor, dsStep.msgOps;
       if actor == idx {
         assert v.Last().hosts[idx].HasKey(k);  // trigger
-      }
-    }
-  }
-}
-
-lemma InvNextAtMostOneInFlight(c: Constants, v: Variables, v': Variables)
-  requires v'.WF(c)
-  requires Inv(c, v)
-  requires Next(c, v, v')
-  ensures AtMostOneInFlight(c, v')
-{
-  forall k, m1, m2 | KeyInFlightByMessage(c, v', m1, k) && KeyInFlightByMessage(c, v', m2, k) 
-  ensures m1 == m2
-  {
-    if m1 != m2 {
-      if KeyInFlightByMessage(c, v, m1, k) {
-        InvNextAtMostOneInFlightHelper(c, v, v', m1, m2, k);
-      } else {
-        InvNextAtMostOneInFlightHelper(c, v, v', m2, m1, k);
-      }
-    }
-  }
-}
-
-lemma InvNextAtMostOneInFlightHelper(c: Constants, v: Variables, v': Variables, m1: Message, m2: Message, k: UniqueKey)
-  requires v'.WF(c)
-  requires Inv(c, v)
-  requires Next(c, v, v')
-  // input constraints
-  requires m1 != m2
-  requires KeyInFlightByMessage(c, v, m1, k)
-  requires !KeyInFlightByMessage(c, v, m2, k)
-  // postcondition
-  ensures !KeyInFlightByMessage(c, v', m2, k)
-{
-  assert KeyInFlight(c, v, k);
-}
-
-lemma InvNextLiveKeyImpliesNoneInFlight(c: Constants, v: Variables, v': Variables)
-  requires v'.WF(c)
-  requires HostsCompleteKeys(c, v')
-  requires Inv(c, v)
-  requires Next(c, v, v')
-  ensures LiveKeyImpliesNoneInFlight(c, v')
-{
-  forall k | !NoneHasLiveKey(c, v', k)
-  ensures !KeyInFlight(c, v', k)
-  {
-    forall msg | msg in v'.network.sentMsgs && k in msg.vks
-    ensures !KeyInFlightByMessage(c, v', msg, k) {
-      var idx :| c.ValidIdx(idx) && v'.Last().hosts[idx].HasLiveKey(k);
-      if v.Last().hosts[idx].HasLiveKey(k) {
-        // triggers
-        assert !KeyInFlight(c, v, k);
-        assert !KeyInFlightByMessage(c, v, msg, k);
-      } else {
-        if msg in v.network.sentMsgs {
-          if KeyInFlightByMessage(c, v, msg, k) {
-            var dsStep :| NextStep(c, v.Last(), v'.Last(), v.network, v'.network, dsStep);
-            var actor, msgOps := dsStep.actor, dsStep.msgOps;
-            // triggers
-            assert KeyInFlightByMessage(c, v, msgOps.recv.value, k);
-            assert KeyInFlight(c, v, k);
-          }
-        }
       }
     }
   }
@@ -235,6 +133,5 @@ lemma AtMostOneHostHasLiveKey(c: Constants, v: Variables, v': Variables, k: Uniq
     }    
   }
 }
-
 
 } // end module ShardedKVProof
