messageInvariantPrototypes/shardedKvBatched/distributedMonotonic/uniquenessInvariants.dfy
@@ -1,0 +1,138 @@
+include "spec.dfy"
+
+module UniquenessInvariants {
+  import opened Types
+  import opened UtilitiesLibrary
+  import opened DistributedSystem
+
+  ghost predicate KeyInFlight(c: Constants, v: Variables, k: UniqueKey) 
+    requires v.WF(c)
+  {
+    exists msg :: KeyInFlightByMessage(c, v, msg, k)
+  }
+
+  ghost predicate KeyInFlightByMessage(c: Constants, v: Variables, msg: Message, k: UniqueKey) 
+    requires v.WF(c)
+  {
+    && msg in v.network.sentMsgs
+    && (0 <= msg.Dst() < |c.hosts| ==>
+      Host.UniqueKeyInFlight(c.hosts[msg.Dst()], v.Last().hosts[msg.Dst()], k, msg)
+    )
+  }
+
+  ghost predicate AtMostOneInFlight(c: Constants, v: Variables)
+    requires v.WF(c)
+  {
+    forall k, m1, m2 | KeyInFlightByMessage(c, v, m1, k) && KeyInFlightByMessage(c, v, m2, k) 
+    :: m1 == m2
+  }
+
+  ghost predicate NoHostOwnsKey(c: Constants, v: Variables, k: UniqueKey) 
+    requires v.WF(c)
+  {
+    forall idx | c.ValidIdx(idx) :: !Host.HostOwnsKey(c.hosts[idx], v.Last().hosts[idx], k)
+  }
+
+  ghost predicate HostOwnsKeyImpliesNoneInFlight(c: Constants, v: Variables)
+    requires v.WF(c)
+  {
+    forall k | !NoHostOwnsKey(c, v, k)
+    ::
+    !KeyInFlight(c, v, k)
+  }
+
+  
+  ghost predicate UniquenessInv(c: Constants, v: Variables)
+    requires v.WF(c)
+  {
+    && AtMostOneInFlight(c, v)
+    && HostOwnsKeyImpliesNoneInFlight(c, v)
+  }
+
+  ghost predicate Inv(c: Constants, v: Variables)
+  {
+    && v.WF(c)
+    && UniquenessInv(c, v)
+  }
+
+  lemma InitImpliesUniquenessInv(c: Constants, v: Variables)
+    requires Init(c, v)
+    ensures Inv(c, v)
+  {}
+
+  lemma UniquenessInvInductive(c: Constants, v: Variables, v': Variables)
+    requires Inv(c, v)
+    requires Next(c, v, v')
+    ensures Inv(c, v')
+  {
+    InvNextAtMostOneInFlight(c, v, v');
+    InvNextLiveKeyImpliesNoneInFlight(c, v, v');
+  }
+
+
+/***************************************************************************************
+*                                 InvNext Proofs                                       *
+***************************************************************************************/
+
+
+lemma InvNextAtMostOneInFlight(c: Constants, v: Variables, v': Variables)
+  requires v'.WF(c)
+  requires Inv(c, v)
+  requires Next(c, v, v')
+  ensures AtMostOneInFlight(c, v')
+{
+  forall k, m1, m2 | KeyInFlightByMessage(c, v', m1, k) && KeyInFlightByMessage(c, v', m2, k) 
+  ensures m1 == m2
+  {
+    if m1 != m2 {
+      if KeyInFlightByMessage(c, v, m1, k) {
+        InvNextAtMostOneInFlightHelper(c, v, v', m1, m2, k);
+      } else {
+        InvNextAtMostOneInFlightHelper(c, v, v', m2, m1, k);
+      }
+    }
+  }
+}
+
+lemma InvNextAtMostOneInFlightHelper(c: Constants, v: Variables, v': Variables, m1: Message, m2: Message, k: UniqueKey)
+  requires v'.WF(c)
+  requires Inv(c, v)
+  requires Next(c, v, v')
+  // input constraints
+  requires m1 != m2
+  requires KeyInFlightByMessage(c, v, m1, k)
+  requires !KeyInFlightByMessage(c, v, m2, k)
+  // postcondition
+  ensures !KeyInFlightByMessage(c, v', m2, k)
+{
+  assert KeyInFlight(c, v, k);
+}
+
+lemma InvNextLiveKeyImpliesNoneInFlight(c: Constants, v: Variables, v': Variables)
+  requires v'.WF(c)
+  requires Inv(c, v)
+  requires Next(c, v, v')
+  ensures HostOwnsKeyImpliesNoneInFlight(c, v')
+{
+  forall k | !NoHostOwnsKey(c, v', k)
+  ensures !KeyInFlight(c, v', k)
+  {
+    forall msg | msg in v'.network.sentMsgs
+    ensures !KeyInFlightByMessage(c, v', msg, k) {
+      var idx :| c.ValidIdx(idx) && Host.HostOwnsKey(c.hosts[idx], v'.Last().hosts[idx], k);
+      if Host.HostOwnsKey(c.hosts[idx], v.Last().hosts[idx], k){
+        // triggers
+        assert !KeyInFlight(c, v, k);
+        assert !KeyInFlightByMessage(c, v, msg, k);
+      } else {
+        if msg in v.network.sentMsgs && KeyInFlightByMessage(c, v, msg, k){
+          var dsStep :| NextStep(c, v.Last(), v'.Last(), v.network, v'.network, dsStep);
+          // triggers
+          assert KeyInFlightByMessage(c, v, dsStep.msgOps.recv.value, k);
+          assert KeyInFlight(c, v, k);
+        }
+      }
+    }
+  }
+}
+} // end module ShardedKVProof
